libcrux-ml-dsa/proofs/fstar/extraction/Libcrux_ml_dsa.Simd.Traits.fst
@@ -4,5 +4,5 @@ open Core
 open FStar.Mul
 
 let int_in_i32_range (i: Hax_lib.Int.t_Int) =
-  i <= (Rust_primitives.Hax.Int.from_machine Core.Num.impl__i32__MAX <: Hax_lib.Int.t_Int) &&
-  i >= (Rust_primitives.Hax.Int.from_machine Core.Num.impl__i32__MIN <: Hax_lib.Int.t_Int)
+  i <= (Rust_primitives.Hax.Int.from_machine Core.Num.impl_i32__MAX <: Hax_lib.Int.t_Int) &&
+  i >= (Rust_primitives.Hax.Int.from_machine Core.Num.impl_i32__MIN <: Hax_lib.Int.t_Int)
