libcrux-ml-dsa/proofs/fstar/extraction/Libcrux_ml_dsa.Simd.Avx2.Encoding.T1.fsti
@@ -6,7 +6,7 @@ open FStar.Mul
 val serialize (simd_unit: Libcrux_intrinsics.Avx2_extract.t_Vec256) (out: t_Slice u8)
     : Prims.Pure (t_Slice u8) Prims.l_True (fun _ -> Prims.l_True)
 
-let deserialize__COEFFICIENT_MASK: i32 = (mk_i32 1 <<! mk_i32 10 <: i32) -! mk_i32 1
+let deserialize__v_COEFFICIENT_MASK: i32 = (mk_i32 1 <<! mk_i32 10 <: i32) -! mk_i32 1
 
 val deserialize (bytes: t_Slice u8) (out: Libcrux_intrinsics.Avx2_extract.t_Vec256)
     : Prims.Pure Libcrux_intrinsics.Avx2_extract.t_Vec256 Prims.l_True (fun _ -> Prims.l_True)
